Algebraic/LowerBound/Fusion.lean
@@ -6,6 +6,7 @@ import Algebraic.LowerBound.Fusion.Arithmetic.MonotonePolynomial
 import Algebraic.LowerBound.Fusion.Arithmetic.MonotonePolynomial.Layer
 import Algebraic.LowerBound.Fusion.Arithmetic.Progress
 import Algebraic.LowerBound.Fusion.Arithmetic.Progress.Separated
+import Algebraic.LowerBound.Fusion.Arithmetic.Progress.Separated.Expansion
 import Algebraic.LowerBound.Fusion.Arithmetic
 import Algebraic.LowerBound.Fusion.Arithmetic.Degree
 import Algebraic.LowerBound.Fusion.SumOfTerms
